\begin{align*}
    \mathbf{F}_{\textrm{C}} & = \mathbf{F}_{\textrm{CA}} + \mathbf{F}_{\textrm{CB}}\\
    \mathbf{F}_{\textrm{CA}} & = \frac{1}{4 \pi \varepsilon_0} \frac{-7q^2 \del{-a \mathbf{e}_x - a \mathbf{e}_y}}{\del{2a^2}^{3/2}}\\
    & = \frac{1}{4 \pi \varepsilon_0} \frac{7q^2 \del{\mathbf{e}_x + \mathbf{e}_y}}{2 \sqrt{2} a^2}\\
    \mathbf{F}_{\textrm{CB}} & = \frac{1}{4 \pi \varepsilon_0} \frac{-q^2 \del{-a \mathbf{e}_e + a \mathbf{e}_y}}{\del{2a^2}^{3/2}}\\
    & = \frac{1}{4 \pi \varepsilon_0} \frac{-q^2 \del{- \mathbf{e}_x + \mathbf{e}_y}}{2 \sqrt{2} a^2}\\
    \mathbf{F}_{\textrm{C}} & = \frac{1}{4 \pi \varepsilon_0} \frac{1}{2 \sqrt{2} a^2} \del{7q^2 \del{\mathbf{e}_x + \mathbf{e}_y} - q^2 \del{- \mathbf{e}_x + \mathbf{e}_y}}\\
    & = \frac{1}{4 \pi \varepsilon_0} \frac{q^2}{2 \sqrt{2} a^2} \del{7 \mathbf{e}_x + 7 \mathbf{e}_y + \mathbf{e}_x - \mathbf{e}_y}\\
    & = \frac{1}{4 \pi \varepsilon_0} \frac{q^2}{2 \sqrt{2} a^2} \del{8 \mathbf{e}_x + 6 \mathbf{e}_y}\\
    & = \frac{q^2}{4 \sqrt{2} \pi \varepsilon_0 a^2} \del{4 \mathbf{e}_x + 3 \mathbf{e}_y}\\
    & = \frac{5q^2}{4 \sqrt{2} \pi \varepsilon_0 a^2} \del{\tfrac{4}{5} \mathbf{e}_x + \tfrac{3}{5} \mathbf{e}_y}
\end{align*}
shrug
